dataplane/LList_Haskell_Setup.thy
@@ -6,22 +6,207 @@ imports
   "Timely_Infrastructure"
 begin
 
-(* code_printing code_module "Deter" \<rightharpoonup> (Haskell)
-  \<open>
-module Deter (cthe_elem, Cset (..) ) where
 
-newtype Cset a = Cset_of_llist [a];
+lemma one_minus[code]:
+  "(1 :: 1) - x = 1"
+  by auto
+lemma one_plus[code]:
+  "(1 :: 1) + x = 1"
+  by auto
 
-cthe_elem (Cset_of_llist xs) = Prelude.head xs;
-\<close>
- *)
+partial_function (llist) lrmdups_aux where
+  "lrmdups_aux f S lxs = (case lxs of LNil \<Rightarrow> LNil | LCons x lxs \<Rightarrow> (if f x \<in> S then lrmdups_aux f S lxs else LCons x (lrmdups_aux f (insert (f x) S) lxs)))"
+declare lrmdups_aux.simps[code]
+
+definition "lrmdups f = lrmdups_aux f {}"
+
+definition "crmdups (f :: 'a \<Rightarrow> 'b) (C :: 'a cset) = C"
+declare crmdups_def[code del]
+
+lemma crmdups_code[code]:
+  "crmdups f (cset_of_llist xs) = cset_of_llist (lrmdups f xs)"
+  sorry
+
+definition "compress_cfilter P xs = cfilter P xs"
+
+friend_of_corec lappend where
+  "lappend xs lys = (case xs of LNil \<Rightarrow> (case lys of LNil \<Rightarrow> LNil | LCons x xs \<Rightarrow> LCons x xs)
+    | LCons x xs \<Rightarrow> LCons x (lappend xs lys))"
+  subgoal by (cases xs; cases lys; simp)
+  subgoal by transfer_prover
+  done
+
+declare csome_elem_def[code del]
+declare cthe_elem_def[code del]
+
+
+definition "csingleton (xs :: 'm cset) = xs"
+declare csingleton_def[code del]
+
+definition "cnub (C :: (_ :: equal) cset) = C"
+declare cnub_def[code del]
+
+definition "ctake (n :: nat) (C :: (_ :: equal) cset) = C"
+declare ctake_def[code del]
+
+
+code_printing code_module "Cset" \<rightharpoonup> (Haskell)
+\<open>
+module Cset (csingleton, chd, Cset (..), Nat (..), cnub, clast, ctake, safe_nth, ndrop, ntake) where
+import qualified Data.List;
+
+newtype Cset a = Cset [a];
+newtype Nat = Nat Integer;
+
+csingleton (Cset []) = Cset [];
+csingleton (Cset xs) = Cset [Prelude.head xs];
+
+chd (Cset xs) = Prelude.head xs;
+clast (Cset xs) = Prelude.last xs;
+
+cnub (Cset xs) = Cset (Data.List.nub xs);
+
+safe_nth xs n = xs !! ((mod (Prelude.fromInteger n) (length  xs)));
+
+ctake (Nat n) (Cset xs) = Cset (Prelude.take (Prelude.fromInteger n) xs);
+
+ndrop (Nat n) xs = drop (Prelude.fromInteger n) xs;
+ntake (Nat n) xs = take (Prelude.fromInteger n) xs;
+
+\<close> 
+
+declare ltaken.simps[code del]
+
+code_printing
+  type_constructor cset \<rightharpoonup>
+    (Haskell) "Cset.Cset _"
+  | type_constructor nat \<rightharpoonup>
+    (Haskell) "Cset.Nat"
+  | constant Nat \<rightharpoonup>
+    (Haskell) "Cset.Nat"
+  | constant cset_of_llist \<rightharpoonup>
+    (Haskell) "Cset.Cset"
+  | constant csingleton \<rightharpoonup>
+    (Haskell) "Cset.csingleton"
+  | constant cthe_elem \<rightharpoonup>
+    (Haskell) "Cset.chd"
+  | constant csome_elem \<rightharpoonup>
+    (Haskell) "Cset.clast"
+  | constant cnub \<rightharpoonup>
+    (Haskell) "Cset.cnub"
+  | constant ctake \<rightharpoonup>
+    (Haskell) "Cset.ctake"
+  | type_constructor llist \<rightharpoonup>
+    (Haskell) "![(_)]"
+  | constant LNil \<rightharpoonup>
+    (Haskell) "[]"
+  | constant LCons \<rightharpoonup>
+    (Haskell) infix 3 ":"
+  | class_instance llist :: equal \<rightharpoonup>
+    (Haskell) -
+  | constant "HOL.equal :: 'a llist \<Rightarrow> 'a llist \<Rightarrow> bool" \<rightharpoonup>
+    (Haskell) infix 4 "=="
+  | constant "lappend" \<rightharpoonup>
+    (Haskell) infixr 5 "++"
+  | constant lmap \<rightharpoonup>
+    (Haskell) "map"
+
+  | constant lfilter \<rightharpoonup>
+    (Haskell) "filter"
+  | constant lconcat \<rightharpoonup>
+    (Haskell) "Prelude.concat"
+  | constant lmerge \<rightharpoonup>
+    (Haskell) "Prelude.concat"
+  | constant lhd \<rightharpoonup>
+    (Haskell) "Prelude.head"
+  | constant hd \<rightharpoonup>
+    (Haskell) "Prelude.head"
+  | constant ltl \<rightharpoonup>
+    (Haskell) "Prelude.tail"
+  | constant tl \<rightharpoonup>
+    (Haskell) "Prelude.tail"
+  | constant last \<rightharpoonup>
+    (Haskell) "Prelude.last"
+  | constant lzip \<rightharpoonup>
+    (Haskell) "zip"
+  | constant llist.lnull \<rightharpoonup>
+    (Haskell) "null"
+  | constant ltakeWhile \<rightharpoonup>
+    (Haskell) "takeWhile"
+  | constant ldropWhile \<rightharpoonup>
+    (Haskell) "dropWhile"
+  | constant ldropn \<rightharpoonup>
+    (Haskell) "Cset.ndrop"
+  | constant ldrop \<rightharpoonup>
+    (Haskell) "Cset.ndrop"
+  | constant ltaken \<rightharpoonup>
+    (Haskell) "Cset.ntake"
+  | constant llist_all \<rightharpoonup>
+    (Haskell) "all"
+  | constant llist_of \<rightharpoonup>
+    (Haskell) "id"
 
 
 
-(*    | constant sum_list \<rightharpoonup>
-    (Haskell) "sum"  *)
-(*   | constant fold \<rightharpoonup>
-    (Haskell) "(\\f xs x -> Prelude.foldl f x xs)"
- *)
+fun wsteps_at :: "('i, 'o, 'd :: countable) op \<Rightarrow> _" where
+  "wsteps_at (Write op p x) n = {|(VOut p x, op)|}"
+| "wsteps_at (Read p f) n = cimage (\<lambda>x. (VInp p x, f x)) (cUNIV :: 'd cset)"
+| "wsteps_at (Silent op) (Suc n) = wsteps_at op n"
+| "wsteps_at (Choice ops) (Suc n) = cUnion (cimage (\<lambda> op. wsteps_at op n) ops)"
+| "wsteps_at op 0 = {||}"
+
+definition "wsteps_exec op = cUnion (cimage (wsteps_at op) cUNIV)"
+
+lemma wsteps_exec_Write[simp]: "wsteps_exec (Write op p x) = {|(VOut p x, op)|}"
+  unfolding wsteps_exec_def by (auto simp: cset_eq_iff)
+
+lemma wsteps_exec_Read[simp]: "wsteps_exec (Read p f) = cimage (\<lambda>x. (VInp p x, f x)) (cUNIV :: _ cset)"
+  unfolding wsteps_exec_def by (auto simp: cset_eq_iff)
+
+lemma wsteps_exec_Silent[simp]:
+  "wsteps_exec (Silent op) = wsteps_exec op"
+  unfolding wsteps_exec_def
+  apply safe
+  subgoal premises prems for a b n
+    using prems(2-) apply -
+    apply (induct "Silent op" n arbitrary: op rule: wsteps_at.induct)
+     apply auto
+    done
+  subgoal for a b n
+    apply (simp add: wsteps_exec_def)
+    apply (rule exI[of _ "Suc n"])
+    apply auto
+    done
+  done
+
+lemma wsteps_exec_Choice[simp]:
+  "wsteps_exec (Choice ops) = cUnion (wsteps_exec |`| ops)"
+  unfolding wsteps_exec_def
+  apply safe
+  subgoal premises prems for a b n
+    using prems(2-) apply -
+    apply (induct "Choice ops" n arbitrary: ops rule: wsteps_at.induct)
+     apply auto
+    done
+  subgoal for a b x n
+    apply (simp add: wsteps_exec_def)
+    apply (rule exI[of _ "Suc n"])
+    apply auto
+    done
+  done
+
+declare wsteps_exec_def[code del]
+lemmas wsteps_exec_code[code] = wsteps_exec_Read wsteps_exec_Write wsteps_exec_Silent wsteps_exec_Choice
+
+
+corec trace_exec where
+  "trace_exec op = (let ops = wsteps_exec op in                      
+   if \<not> cis_empty ops then let (io, op') = cthe_elem ops in LCons io (trace_exec op')
+   else LNil)"
+
+lemma acset_code[code]:
+  "acset S = cset_of_llist (lfilter (\<lambda> x. x \<in> S) cenum)"
+  unfolding cset_of_llist_def map_fun_def o_apply id_apply using UNIV_cenum by auto
+
 
 end
